Progress on TImp

dsss17/TImp.v
@@ -53,34 +53,35 @@ Theorem false_beq_id : forall x y : id,
    -> beq_id x y = false.
 Admitted. (* QuickChick false_beq_id. *)
 
-Definition partial_map := list (id * nat).
+Inductive value := VNat : nat -> value | VBool : bool -> value.
+
+Definition partial_map := list (id * value).
 
 Definition empty : partial_map := nil.
 
-Definition update := @cons (id * nat).
+Definition update := @cons (id * value).
 
-Inductive bind : partial_map -> id -> nat -> Prop :=
+Inductive bind : partial_map -> id -> value -> Prop :=
   | BindNow   : forall x a m, bind (cons (x, a) m) x a
   | BindLater : forall x x' a a' m',
                   ~ (x = x') ->
                   bind m' x a -> 
                   bind (cons (x',a') m') x a.
 
+(* DELETE -- write by hand *)
 Derive ArbitrarySizedSuchThat for (fun x => bind m x a).
-Derive SizeMonotonicSuchThatOpt for (fun x => bind m x a).
 
-(* ZOE!
-Derive SizedProofEqs for (fun x => bind m x a).
-Derive GenSizedSuchThatCorrect for (fun x => bind m x a).
-Derive GenSizedSuchThatSizeMonotonicOpt for (fun x => bind m x a).
-*)
+(* NOT NEEDED
 Instance adm_st m a : SuchThatCorrect (fun x => bind m x a) (genST (fun x => bind m x a)).
 Admitted.
+*)
 
+(* MOVE TO QC *)
 Instance checkFalse : Checkable False := {| checker := fun _ => checker false |}.
 
 Instance bind_dec m x v : Dec (bind m x v) :=
   {| dec := _ |}.
+(* remove ssr...
 Proof.
   move: x v.
   induction m => x v.
@@ -96,6 +97,7 @@ Proof.
       * left; constructor; eauto.
       * right => Contra; inversion Contra; subst; eauto.
 Defined.
+*) Admitted.
 
 (* TODO: Correct equivalence of maps *)
 Definition equiv_map m1 m2 :=
@@ -108,6 +110,9 @@ Conjecture apply_empty : forall x a, ~ (bind empty x a).
 Conjecture update_eq : forall (m: partial_map) x v,
     bind (update (x,v) m) x v.
 (* QuickChick update_eq. *)
+
+(* TODO: Change it to equivalence === -- use Equivalence
+   typeclass?  (These are sadly false at the moment) *)
 
 Theorem update_neq : forall v x1 x2
                        (m : partial_map),
@@ -150,858 +155,20 @@ Module AExp.
 (** These two definitions specify the _abstract syntax_ of
     arithmetic and boolean expressions. *)
 
-Inductive aexp : Type :=
-  | ANum : nat -> aexp
-  | APlus : aexp -> aexp -> aexp
-  | AMinus : aexp -> aexp -> aexp
-  | AMult : aexp -> aexp -> aexp.
-
-Inductive bexp : Type :=
-  | BTrue : bexp
-  | BFalse : bexp
-  | BEq : aexp -> aexp -> bexp
-  | BLe : aexp -> aexp -> bexp
-  | BNot : bexp -> bexp
-  | BAnd : bexp -> bexp -> bexp.
-
-(** In this chapter, we'll elide the translation from the
-    concrete syntax that a programmer would actually write to these
-    abstract syntax trees -- the process that, for example, would
-    translate the string ["1+2*3"] to the AST
-
-      APlus (ANum 1) (AMult (ANum 2) (ANum 3)).
-
-    The optional chapter [ImpParser] develops a simple
-    implementation of a lexical analyzer and parser that can perform
-    this translation.  You do _not_ need to understand that chapter to
-    understand this one, but if you haven't taken a course where these
-    techniques are covered (e.g., a compilers course) you may want to
-    skim it. *)
-
-(** For comparison, here's a conventional BNF (Backus-Naur Form)
-    grammar defining the same abstract syntax:
-
-    a ::= nat
-        | a + a
-        | a - a
-        | a * a
-
-    b ::= true
-        | false
-        | a = a
-        | a <= a
-        | not b
-        | b and b
-*)
-
-(** Compared to the Coq version above...
-
-       - The BNF is more informal -- for example, it gives some
-         suggestions about the surface syntax of expressions (like the
-         fact that the addition operation is written [+] and is an
-         infix symbol) while leaving other aspects of lexical analysis
-         and parsing (like the relative precedence of [+], [-], and
-         [*], the use of parens to explicitly group subexpressions,
-         etc.) unspecified.  Some additional information (and human
-         intelligence) would be required to turn this description into
-         a formal definition, for example when implementing a
-         compiler.
-
-         The Coq version consistently omits all this information and
-         concentrates on the abstract syntax only.
-
-       - On the other hand, the BNF version is lighter and easier to
-         read.  Its informality makes it flexible, a big advantage in
-         situations like discussions at the blackboard, where
-         conveying general ideas is more important than getting every
-         detail nailed down precisely.
-
-         Indeed, there are dozens of BNF-like notations and people
-         switch freely among them, usually without bothering to say
-         which form of BNF they're using because there is no need to:
-         a rough-and-ready informal understanding is all that's
-         important.
-
-    It's good to be comfortable with both sorts of notations: informal
-    ones for communicating between humans and formal ones for carrying
-    out implementations and proofs. *)
-
-(* ================================================================= *)
-(** ** Evaluation *)
-
-(** _Evaluating_ an arithmetic expression produces a number. *)
-
-Fixpoint aeval (a : aexp) : nat :=
-  match a with
-  | ANum n => n
-  | APlus a1 a2 => (aeval a1) + (aeval a2)
-  | AMinus a1 a2  => (aeval a1) - (aeval a2)
-  | AMult a1 a2 => (aeval a1) * (aeval a2)
-  end.
-
-Example test_aeval1:
-  aeval (APlus (ANum 2) (ANum 2)) = 4.
-Proof. reflexivity. Qed.
-
-(** Similarly, evaluating a boolean expression yields a boolean. *)
-
-Fixpoint beval (b : bexp) : bool :=
-  match b with
-  | BTrue       => true
-  | BFalse      => false
-  | BEq a1 a2   => beq_nat (aeval a1) (aeval a2)
-  | BLe a1 a2   => leb (aeval a1) (aeval a2)
-  | BNot b1     => negb (beval b1)
-  | BAnd b1 b2  => andb (beval b1) (beval b2)
-  end.
-
-(* ================================================================= *)
-(** ** Optimization *)
-
-(** We haven't defined very much yet, but we can already get
-    some mileage out of the definitions.  Suppose we define a function
-    that takes an arithmetic expression and slightly simplifies it,
-    changing every occurrence of [0+e] (i.e., [(APlus (ANum 0) e])
-    into just [e]. *)
-
-Fixpoint optimize_0plus (a:aexp) : aexp :=
-  match a with
-  | ANum n =>
-      ANum n
-  | APlus (ANum 0) e2 =>
-      optimize_0plus e2
-  | APlus e1 e2 =>
-      APlus (optimize_0plus e1) (optimize_0plus e2)
-  | AMinus e1 e2 =>
-      AMinus (optimize_0plus e1) (optimize_0plus e2)
-  | AMult e1 e2 =>
-      AMult (optimize_0plus e1) (optimize_0plus e2)
-  end.
-
-(** To make sure our optimization is doing the right thing we
-    can test it on some examples and see if the output looks OK. *)
-
-Example test_optimize_0plus:
-  optimize_0plus (APlus (ANum 2)
-                        (APlus (ANum 0)
-                               (APlus (ANum 0) (ANum 1))))
-  = APlus (ANum 2) (ANum 1).
-Proof. reflexivity. Qed.
-
-(** But if we want to be sure the optimization is correct --
-    i.e., that evaluating an optimized expression gives the same
-    result as the original -- we should prove it. *)
-
-Theorem optimize_0plus_sound: forall a,
-  aeval (optimize_0plus a) = aeval a.
-Proof.
-  intros a. induction a.
-  - (* ANum *) reflexivity.
-  - (* APlus *) destruct a1.
-    + (* a1 = ANum n *) destruct n.
-      * (* n = 0 *)  simpl. apply IHa2.
-      * (* n <> 0 *) simpl. rewrite IHa2. reflexivity.
-    + (* a1 = APlus a1_1 a1_2 *)
-      simpl. simpl in IHa1. rewrite IHa1.
-      rewrite IHa2. reflexivity.
-    + (* a1 = AMinus a1_1 a1_2 *)
-      simpl. simpl in IHa1. rewrite IHa1.
-      rewrite IHa2. reflexivity.
-    + (* a1 = AMult a1_1 a1_2 *)
-      simpl. simpl in IHa1. rewrite IHa1.
-      rewrite IHa2. reflexivity.
-  - (* AMinus *)
-    simpl. rewrite IHa1. rewrite IHa2. reflexivity.
-  - (* AMult *)
-    simpl. rewrite IHa1. rewrite IHa2. reflexivity.  Qed.
-
-(* ################################################################# *)
-(** * Coq Automation *)
-
-(** The amount of repetition in this last proof is a little
-    annoying.  And if either the language of arithmetic expressions or
-    the optimization being proved sound were significantly more
-    complex, it would start to be a real problem.
-
-    So far, we've been doing all our proofs using just a small handful
-    of Coq's tactics and completely ignoring its powerful facilities
-    for constructing parts of proofs automatically.  This section
-    introduces some of these facilities, and we will see more over the
-    next several chapters.  Getting used to them will take some
-    energy -- Coq's automation is a power tool -- but it will allow us
-    to scale up our efforts to more complex definitions and more
-    interesting properties without becoming overwhelmed by boring,
-    repetitive, low-level details. *)
-
-(* ================================================================= *)
-(** ** Tacticals *)
-
-(** _Tacticals_ is Coq's term for tactics that take other tactics as
-    arguments -- "higher-order tactics," if you will.  *)
-
-(* ----------------------------------------------------------------- *)
-(** *** The [try] Tactical *)
-
-(** If [T] is a tactic, then [try T] is a tactic that is just like [T]
-    except that, if [T] fails, [try T] _successfully_ does nothing at
-    all (instead of failing). *)
-
-Theorem silly1 : forall ae, aeval ae = aeval ae.
-Proof. try reflexivity. (* this just does [reflexivity] *) Qed.
-
-Theorem silly2 : forall (P : Prop), P -> P.
-Proof.
-  intros P HP.
-  try reflexivity. (* just [reflexivity] would have failed *)
-  apply HP. (* we can still finish the proof in some other way *)
-Qed.
-
-(** There is no real reason to use [try] in completely manual
-    proofs like these, but it is very useful for doing automated
-    proofs in conjunction with the [;] tactical, which we show
-    next. *)
-
-(* ----------------------------------------------------------------- *)
-(** *** The [;] Tactical (Simple Form) *)
-
-(** In its most common form, the [;] tactical takes two tactics as
-    arguments.  The compound tactic [T;T'] first performs [T] and then
-    performs [T'] on _each subgoal_ generated by [T]. *)
-
-(** For example, consider the following trivial lemma: *)
-
-Lemma foo : forall n, leb 0 n = true.
-Proof.
-  intros.
-  destruct n.
-    (* Leaves two subgoals, which are discharged identically...  *)
-    - (* n=0 *) simpl. reflexivity.
-    - (* n=Sn' *) simpl. reflexivity.
-Qed.
-
-(** We can simplify this proof using the [;] tactical: *)
-
-Lemma foo' : forall n, leb 0 n = true.
-Proof.
-  intros.
-  (* [destruct] the current goal *)
-  destruct n;
-  (* then [simpl] each resulting subgoal *)
-  simpl;
-  (* and do [reflexivity] on each resulting subgoal *)
-  reflexivity.
-Qed.
-
-(** Using [try] and [;] together, we can get rid of the repetition in
-    the proof that was bothering us a little while ago. *)
-
-Theorem optimize_0plus_sound': forall a,
-  aeval (optimize_0plus a) = aeval a.
-Proof.
-  intros a.
-  induction a;
-    (* Most cases follow directly by the IH... *)
-    try (simpl; rewrite IHa1; rewrite IHa2; reflexivity).
-    (* ... but the remaining cases -- ANum and APlus --
-       are different: *)
-  - (* ANum *) reflexivity.
-  - (* APlus *)
-    destruct a1;
-      (* Again, most cases follow directly by the IH: *)
-      try (simpl; simpl in IHa1; rewrite IHa1;
-           rewrite IHa2; reflexivity).
-    (* The interesting case, on which the [try...]
-       does nothing, is when [e1 = ANum n]. In this
-       case, we have to destruct [n] (to see whether
-       the optimization applies) and rewrite with the
-       induction hypothesis. *)
-    + (* a1 = ANum n *) destruct n;
-      simpl; rewrite IHa2; reflexivity.   Qed.
-
-(** Coq experts often use this "[...; try... ]" idiom after a tactic
-    like [induction] to take care of many similar cases all at once.
-    Naturally, this practice has an analog in informal proofs.  For
-    example, here is an informal proof of the optimization theorem
-    that matches the structure of the formal one:
-
-    _Theorem_: For all arithmetic expressions [a],
-
-       aeval (optimize_0plus a) = aeval a.
-
-    _Proof_: By induction on [a].  Most cases follow directly from the
-    IH.  The remaining cases are as follows:
-
-      - Suppose [a = ANum n] for some [n].  We must show
-
-          aeval (optimize_0plus (ANum n)) = aeval (ANum n).
-
-        This is immediate from the definition of [optimize_0plus].
-
-      - Suppose [a = APlus a1 a2] for some [a1] and [a2].  We must
-        show
-
-          aeval (optimize_0plus (APlus a1 a2)) = aeval (APlus a1 a2).
-
-        Consider the possible forms of [a1].  For most of them,
-        [optimize_0plus] simply calls itself recursively for the
-        subexpressions and rebuilds a new expression of the same form
-        as [a1]; in these cases, the result follows directly from the
-        IH.
-
-        The interesting case is when [a1 = ANum n] for some [n].  If
-        [n = ANum 0], then
-
-          optimize_0plus (APlus a1 a2) = optimize_0plus a2
-
-        and the IH for [a2] is exactly what we need.  On the other
-        hand, if [n = S n'] for some [n'], then again [optimize_0plus]
-        simply calls itself recursively, and the result follows from
-        the IH.  [] *)
-
-(** However, this proof can still be improved: the first case (for
-    [a = ANum n]) is very trivial -- even more trivial than the cases
-    that we said simply followed from the IH -- yet we have chosen to
-    write it out in full.  It would be better and clearer to drop it
-    and just say, at the top, "Most cases are either immediate or
-    direct from the IH.  The only interesting case is the one for
-    [APlus]..."  We can make the same improvement in our formal proof
-    too.  Here's how it looks: *)
-
-Theorem optimize_0plus_sound'': forall a,
-  aeval (optimize_0plus a) = aeval a.
-Proof.
-  intros a.
-  induction a;
-    (* Most cases follow directly by the IH *)
-    try (simpl; rewrite IHa1; rewrite IHa2; reflexivity);
-    (* ... or are immediate by definition *)
-    try reflexivity.
-  (* The interesting case is when a = APlus a1 a2. *)
-  - (* APlus *)
-    destruct a1; try (simpl; simpl in IHa1; rewrite IHa1;
-                      rewrite IHa2; reflexivity).
-    + (* a1 = ANum n *) destruct n;
-      simpl; rewrite IHa2; reflexivity. Qed.
-
-(* ----------------------------------------------------------------- *)
-(** *** The [;] Tactical (General Form) *)
-
-(** The [;] tactical also has a more general form than the simple
-    [T;T'] we've seen above.  If [T], [T1], ..., [Tn] are tactics,
-    then
-
-      T; [T1 | T2 | ... | Tn]
-
-   is a tactic that first performs [T] and then performs [T1] on the
-   first subgoal generated by [T], performs [T2] on the second
-   subgoal, etc.
-
-   So [T;T'] is just special notation for the case when all of the
-   [Ti]'s are the same tactic; i.e., [T;T'] is shorthand for:
-
-      T; [T' | T' | ... | T']
-*)
-
-(* ----------------------------------------------------------------- *)
-(** *** The [repeat] Tactical *)
-
-(** The [repeat] tactical takes another tactic and keeps applying this
-    tactic until it fails. Here is an example showing that [10] is in
-    a long list using repeat. *)
-
-Theorem In10 : In 10 [1;2;3;4;5;6;7;8;9;10].
-Proof.
-  repeat (try (left; reflexivity); right).
-Qed.
-
-(** The tactic [repeat T] never fails: if the tactic [T] doesn't apply
-    to the original goal, then repeat still succeeds without changing
-    the original goal (i.e., it repeats zero times). *)
-
-Theorem In10' : In 10 [1;2;3;4;5;6;7;8;9;10].
-Proof.
-  repeat (left; reflexivity).
-  repeat (right; try (left; reflexivity)).
-Qed.
-
-(** The tactic [repeat T] also does not have any upper bound on the
-    number of times it applies [T].  If [T] is a tactic that always
-    succeeds, then repeat [T] will loop forever (e.g., [repeat simpl]
-    loops forever, since [simpl] always succeeds).  While evaluation
-    in Coq's term language, Gallina, is guaranteed to terminate,
-    tactic evaluation is not!  This does not affect Coq's logical
-    consistency, however, since the job of [repeat] and other tactics
-    is to guide Coq in constructing proofs; if the construction
-    process diverges, this simply means that we have failed to
-    construct a proof, not that we have constructed a wrong one. *)
-
-(** **** Exercise: 3 stars (optimize_0plus_b)  *)
-(** Since the [optimize_0plus] transformation doesn't change the value
-    of [aexp]s, we should be able to apply it to all the [aexp]s that
-    appear in a [bexp] without changing the [bexp]'s value.  Write a
-    function which performs that transformation on [bexp]s, and prove
-    it is sound.  Use the tacticals we've just seen to make the proof
-    as elegant as possible. *)
-
-Fixpoint optimize_0plus_b (b : bexp) : bexp
-  (* REPLACE THIS LINE WITH ":= _your_definition_ ." *). Admitted.
-
-Theorem optimize_0plus_b_sound : forall b,
-  beval (optimize_0plus_b b) = beval b.
-Proof.
-  (* FILL IN HERE *) Admitted.
-(** [] *)
-
-(** **** Exercise: 4 stars, optional (optimizer)  *)
-(** _Design exercise_: The optimization implemented by our
-    [optimize_0plus] function is only one of many possible
-    optimizations on arithmetic and boolean expressions.  Write a more
-    sophisticated optimizer and prove it correct.  (You will probably
-    find it easiest to start small -- add just a single, simple
-    optimization and prove it correct -- and build up to something
-    more interesting incrementially.)
-
-(* FILL IN HERE *)
-*)
-(** [] *)
-
-(* ================================================================= *)
-(** ** Defining New Tactic Notations *)
-
-(** Coq also provides several ways of "programming" tactic scripts.
-
-    - The [Tactic Notation] idiom illustrated below gives a handy way to
-      define "shorthand tactics" that bundle several tactics into a
-      single command.
-
-    - For more sophisticated programming, Coq offers a built-in
-      programming language called [Ltac] with primitives that can
-      examine and modify the proof state.  The details are a bit too
-      complicated to get into here (and it is generally agreed that
-      [Ltac] is not the most beautiful part of Coq's design!), but they
-      can be found in the reference manual and other books on Coq, and
-      there are many examples of [Ltac] definitions in the Coq standard
-      library that you can use as examples.
-
-    - There is also an OCaml API, which can be used to build tactics
-      that access Coq's internal structures at a lower level, but this
-      is seldom worth the trouble for ordinary Coq users.
-
-    The [Tactic Notation] mechanism is the easiest to come to grips with,
-    and it offers plenty of power for many purposes.  Here's an example. *)
-
-Tactic Notation "simpl_and_try" tactic(c) :=
-  simpl;
-  try c.
-
-(** This defines a new tactical called [simpl_and_try] that takes one
-    tactic [c] as an argument and is defined to be equivalent to the
-    tactic [simpl; try c].  Now writing "[simpl_and_try reflexivity.]"
-    in a proof will be the same as writing "[simpl; try
-    reflexivity.]" *)
-
-(* ================================================================= *)
-(** ** The [omega] Tactic *)
-
-(** The [omega] tactic implements a decision procedure for a subset of
-    first-order logic called _Presburger arithmetic_.  It is based on
-    the Omega algorithm invented in 1991 by William Pugh [Pugh 1991].
-
-    If the goal is a universally quantified formula made out of
-
-      - numeric constants, addition ([+] and [S]), subtraction ([-]
-        and [pred]), and multiplication by constants (this is what
-        makes it Presburger arithmetic),
-
-      - equality ([=] and [<>]) and inequality ([<=]), and
-
-      - the logical connectives [/\], [\/], [~], and [->],
-
-    then invoking [omega] will either solve the goal or tell you that
-    it is actually false. *)
-
-Example silly_presburger_example : forall m n o p,
-  m + n <= n + o /\ o + 3 = p + 3 ->
-  m <= p.
-Proof.
-  intros. omega.
-Qed.
-
-(** (Note the [Require Import Coq.omega.Omega.] at the top of the file.) *)
-
-(* ================================================================= *)
-(** ** A Few More Handy Tactics *)
-
-(** Finally, here are some miscellaneous tactics that you may find
-    convenient.
-
-     - [clear H]: Delete hypothesis [H] from the context.
-
-     - [subst x]: Find an assumption [x = e] or [e = x] in the
-       context, replace [x] with [e] throughout the context and
-       current goal, and clear the assumption.
-
-     - [subst]: Substitute away _all_ assumptions of the form [x = e]
-       or [e = x].
-
-     - [rename... into...]: Change the name of a hypothesis in the
-       proof context.  For example, if the context includes a variable
-       named [x], then [rename x into y] will change all occurrences
-       of [x] to [y].
-
-     - [assumption]: Try to find a hypothesis [H] in the context that
-       exactly matches the goal; if one is found, behave like [apply
-       H].
-
-     - [contradiction]: Try to find a hypothesis [H] in the current
-       context that is logically equivalent to [False].  If one is
-       found, solve the goal.
-
-     - [constructor]: Try to find a constructor [c] (from some
-       [Inductive] definition in the current environment) that can be
-       applied to solve the current goal.  If one is found, behave
-       like [apply c].
-
-    We'll see examples below. *)
-
-(* ################################################################# *)
-(** * Evaluation as a Relation *)
-
-(** We have presented [aeval] and [beval] as functions defined by
-    [Fixpoint]s.  Another way to think about evaluation -- one that we
-    will see is often more flexible -- is as a _relation_ between
-    expressions and their values.  This leads naturally to [Inductive]
-    definitions like the following one for arithmetic expressions... *)
-
-Module aevalR_first_try.
-
-Inductive aevalR : aexp -> nat -> Prop :=
-  | E_ANum  : forall (n: nat),
-      aevalR (ANum n) n
-  | E_APlus : forall (e1 e2: aexp) (n1 n2: nat),
-      aevalR e1 n1 ->
-      aevalR e2 n2 ->
-      aevalR (APlus e1 e2) (n1 + n2)
-  | E_AMinus: forall (e1 e2: aexp) (n1 n2: nat),
-      aevalR e1 n1 ->
-      aevalR e2 n2 ->
-      aevalR (AMinus e1 e2) (n1 - n2)
-  | E_AMult : forall (e1 e2: aexp) (n1 n2: nat),
-      aevalR e1 n1 ->
-      aevalR e2 n2 ->
-      aevalR (AMult e1 e2) (n1 * n2).
-
-(** It will be convenient to have an infix notation for
-    [aevalR].  We'll write [e \\ n] to mean that arithmetic expression
-    [e] evaluates to value [n]. *)
-
-Notation "e '\\' n"
-         := (aevalR e n)
-            (at level 50, left associativity)
-         : type_scope.
-
-End aevalR_first_try.
-
-(** In fact, Coq provides a way to use this notation in the
-    definition of [aevalR] itself.  This reduces confusion by avoiding
-    situations where we're working on a proof involving statements in
-    the form [e \\ n] but we have to refer back to a definition
-    written using the form [aevalR e n].
-
-    We do this by first "reserving" the notation, then giving the
-    definition together with a declaration of what the notation
-    means. *)
-
-Reserved Notation "e '\\' n" (at level 50, left associativity).
-
-Inductive aevalR : aexp -> nat -> Prop :=
-  | E_ANum : forall (n:nat),
-      (ANum n) \\ n
-  | E_APlus : forall (e1 e2: aexp) (n1 n2 : nat),
-      (e1 \\ n1) -> (e2 \\ n2) -> (APlus e1 e2) \\ (n1 + n2)
-  | E_AMinus : forall (e1 e2: aexp) (n1 n2 : nat),
-      (e1 \\ n1) -> (e2 \\ n2) -> (AMinus e1 e2) \\ (n1 - n2)
-  | E_AMult :  forall (e1 e2: aexp) (n1 n2 : nat),
-      (e1 \\ n1) -> (e2 \\ n2) -> (AMult e1 e2) \\ (n1 * n2)
-
-  where "e '\\' n" := (aevalR e n) : type_scope.
-
-(* ================================================================= *)
-(** ** Inference Rule Notation *)
-
-(** In informal discussions, it is convenient to write the rules for
-    [aevalR] and similar relations in the more readable graphical form
-    of _inference rules_, where the premises above the line justify
-    the conclusion below the line (we have already seen them in the
-    [IndProp] chapter). *)
-
-(** For example, the constructor [E_APlus]...
-
-      | E_APlus : forall (e1 e2: aexp) (n1 n2: nat),
-          aevalR e1 n1 ->
-          aevalR e2 n2 ->
-          aevalR (APlus e1 e2) (n1 + n2)
-
-    ...would be written like this as an inference rule:
-
-                               e1 \\ n1
-                               e2 \\ n2
-                         --------------------                         (E_APlus)
-                         APlus e1 e2 \\ n1+n2
-*)
-
-(** Formally, there is nothing deep about inference rules: they
-    are just implications.  You can read the rule name on the right as
-    the name of the constructor and read each of the linebreaks
-    between the premises above the line (as well as the line itself)
-    as [->].  All the variables mentioned in the rule ([e1], [n1],
-    etc.) are implicitly bound by universal quantifiers at the
-    beginning. (Such variables are often called _metavariables_ to
-    distinguish them from the variables of the language we are
-    defining.  At the moment, our arithmetic expressions don't include
-    variables, but we'll soon be adding them.)  The whole collection
-    of rules is understood as being wrapped in an [Inductive]
-    declaration.  In informal prose, this is either elided or else
-    indicated by saying something like "Let [aevalR] be the smallest
-    relation closed under the following rules...". *)
-
-(** For example, [\\] is the smallest relation closed under these
-    rules:
-
-                             -----------                               (E_ANum)
-                             ANum n \\ n
-
-                               e1 \\ n1
-                               e2 \\ n2
-                         --------------------                         (E_APlus)
-                         APlus e1 e2 \\ n1+n2
-
-                               e1 \\ n1
-                               e2 \\ n2
-                        ---------------------                        (E_AMinus)
-                        AMinus e1 e2 \\ n1-n2
-
-                               e1 \\ n1
-                               e2 \\ n2
-                         --------------------                         (E_AMult)
-                         AMult e1 e2 \\ n1*n2
-*)
-
-(* ================================================================= *)
-(** ** Equivalence of the Definitions *)
-
-(** It is straightforward to prove that the relational and functional
-    definitions of evaluation agree: *)
-
-Theorem aeval_iff_aevalR : forall a n,
-  (a \\ n) <-> aeval a = n.
-Proof.
- split.
- - (* -> *)
-   intros H.
-   induction H; simpl.
-   + (* E_ANum *)
-     reflexivity.
-   + (* E_APlus *)
-     rewrite IHaevalR1.  rewrite IHaevalR2.  reflexivity.
-   + (* E_AMinus *)
-     rewrite IHaevalR1.  rewrite IHaevalR2.  reflexivity.
-   + (* E_AMult *)
-     rewrite IHaevalR1.  rewrite IHaevalR2.  reflexivity.
- - (* <- *)
-   generalize dependent n.
-   induction a;
-      simpl; intros; subst.
-   + (* ANum *)
-     apply E_ANum.
-   + (* APlus *)
-     apply E_APlus.
-      apply IHa1. reflexivity.
-      apply IHa2. reflexivity.
-   + (* AMinus *)
-     apply E_AMinus.
-      apply IHa1. reflexivity.
-      apply IHa2. reflexivity.
-   + (* AMult *)
-     apply E_AMult.
-      apply IHa1. reflexivity.
-      apply IHa2. reflexivity.
-Qed.
-
-(** We can make the proof quite a bit shorter by making more
-    use of tacticals. *)
-
-Theorem aeval_iff_aevalR' : forall a n,
-  (a \\ n) <-> aeval a = n.
-Proof.
-  (* WORKED IN CLASS *)
-  split.
-  - (* -> *)
-    intros H; induction H; subst; reflexivity.
-  - (* <- *)
-    generalize dependent n.
-    induction a; simpl; intros; subst; constructor;
-       try apply IHa1; try apply IHa2; reflexivity.
-Qed.
-
-(** **** Exercise: 3 stars  (bevalR)  *)
-(** Write a relation [bevalR] in the same style as
-    [aevalR], and prove that it is equivalent to [beval].*)
-
-Inductive bevalR: bexp -> bool -> Prop :=
-(* FILL IN HERE *)
-.
-
-Lemma beval_iff_bevalR : forall b bv,
-  bevalR b bv <-> beval b = bv.
-Proof.
-  (* FILL IN HERE *) Admitted.
-(** [] *)
-
-End AExp.
-
-(* ================================================================= *)
-(** ** Computational vs. Relational Definitions *)
-
-(** For the definitions of evaluation for arithmetic and boolean
-    expressions, the choice of whether to use functional or relational
-    definitions is mainly a matter of taste: either way works.
-
-    However, there are circumstances where relational definitions of
-    evaluation work much better than functional ones.  *)
-
-Module aevalR_division.
-
-(** For example, suppose that we wanted to extend the arithmetic
-    operations by considering also a division operation:*)
-
-Inductive aexp : Type :=
-  | ANum : nat -> aexp
-  | APlus : aexp -> aexp -> aexp
-  | AMinus : aexp -> aexp -> aexp
-  | AMult : aexp -> aexp -> aexp
-  | ADiv : aexp -> aexp -> aexp.   (* <--- new *)
-
-(** Extending the definition of [aeval] to handle this new operation
-    would not be straightforward (what should we return as the result
-    of [ADiv (ANum 5) (ANum 0)]?).  But extending [aevalR] is
-    straightforward. *)
-
-Reserved Notation "e '\\' n"
-                  (at level 50, left associativity).
-
-Inductive aevalR : aexp -> nat -> Prop :=
-  | E_ANum : forall (n:nat),
-      (ANum n) \\ n
-  | E_APlus : forall (a1 a2: aexp) (n1 n2 : nat),
-      (a1 \\ n1) -> (a2 \\ n2) -> (APlus a1 a2) \\ (n1 + n2)
-  | E_AMinus : forall (a1 a2: aexp) (n1 n2 : nat),
-      (a1 \\ n1) -> (a2 \\ n2) -> (AMinus a1 a2) \\ (n1 - n2)
-  | E_AMult :  forall (a1 a2: aexp) (n1 n2 : nat),
-      (a1 \\ n1) -> (a2 \\ n2) -> (AMult a1 a2) \\ (n1 * n2)
-  | E_ADiv :  forall (a1 a2: aexp) (n1 n2 n3: nat),
-      (a1 \\ n1) -> (a2 \\ n2) -> (n2 > 0) ->
-      (mult n2 n3 = n1) -> (ADiv a1 a2) \\ n3
-
-where "a '\\' n" := (aevalR a n) : type_scope.
-
-End aevalR_division.
-
-Module aevalR_extended.
-
-(** Suppose, instead, that we want to extend the arithmetic operations
-    by a nondeterministic number generator [any] that, when evaluated,
-    may yield any number.  (Note that this is not the same as making a
-    _probabilistic_ choice among all possible numbers -- we're not
-    specifying any particular distribution of results, but just saying
-    what results are _possible_.) *)
-
-Reserved Notation "e '\\' n" (at level 50, left associativity).
-
-Inductive aexp : Type :=
-  | AAny  : aexp                   (* <--- NEW *)
-  | ANum : nat -> aexp
-  | APlus : aexp -> aexp -> aexp
-  | AMinus : aexp -> aexp -> aexp
-  | AMult : aexp -> aexp -> aexp.
-
-(** Again, extending [aeval] would be tricky, since now evaluation is
-    _not_ a deterministic function from expressions to numbers, but
-    extending [aevalR] is no problem: *)
-
-Inductive aevalR : aexp -> nat -> Prop :=
-  | E_Any : forall (n:nat),
-      AAny \\ n                 (* <--- new *)
-  | E_ANum : forall (n:nat),
-      (ANum n) \\ n
-  | E_APlus : forall (a1 a2: aexp) (n1 n2 : nat),
-      (a1 \\ n1) -> (a2 \\ n2) -> (APlus a1 a2) \\ (n1 + n2)
-  | E_AMinus : forall (a1 a2: aexp) (n1 n2 : nat),
-      (a1 \\ n1) -> (a2 \\ n2) -> (AMinus a1 a2) \\ (n1 - n2)
-  | E_AMult :  forall (a1 a2: aexp) (n1 n2 : nat),
-      (a1 \\ n1) -> (a2 \\ n2) -> (AMult a1 a2) \\ (n1 * n2)
-
-where "a '\\' n" := (aevalR a n) : type_scope.
-
-End aevalR_extended.
-
-(** At this point you maybe wondering: which style should I use by
-    default?  The examples above show that relational definitions are
-    fundamentally more powerful than functional ones.  For situations
-    like these, where the thing being defined is not easy to express
-    as a function, or indeed where it is _not_ a function, there is no
-    choice.  But what about when both styles are workable?
-
-    One point in favor of relational definitions is that some people
-    feel they are more elegant and easier to understand.  Another is
-    that Coq automatically generates nice inversion and induction
-    principles from [Inductive] definitions.
-
-    On the other hand, functional definitions can often be more
-    convenient:
-     - Functions are by definition deterministic and defined on all
-       arguments; for a relation we have to show these properties
-       explicitly if we need them.
-     - With functions we can also take advantage of Coq's computation
-       mechanism to simplify expressions during proofs.
-
-    Furthermore, functions can be directly "extracted" to executable
-    code in OCaml or Haskell.
-
-    Ultimately, the choice often comes down to either the specifics of
-    a particular situation or simply a question of taste.  Indeed, in
-    large Coq developments it is common to see a definition given in
-    _both_ functional and relational styles, plus a lemma stating that
-    the two coincide, allowing further proofs to switch from one point
-    of view to the other at will.*)
-
-(* ################################################################# *)
-(** * Expressions With Variables *)
-
-(** Let's turn our attention back to defining Imp.  The next thing we
-    need to do is to enrich our arithmetic and boolean expressions
-    with variables.  To keep things simple, we'll assume that all
-    variables are global and that they only hold numbers. *)
-
-(* ================================================================= *)
-(** ** States *)
-
-(** Since we'll want to look variables up to find out their current
-    values, we'll reuse the type [id] from the [Maps] chapter for the
-    type of variables in Imp.
-
-    A _machine state_ (or just _state_) represents the current values
-    of _all_ variables at some point in the execution of a program. *)
-
-(** For simplicity, we assume that the state is defined for
-    _all_ variables, even though any given program is only going to
-    mention a finite number of them.  The state captures all of the
-    information stored in memory.  For Imp programs, because each
-    variable stores a natural number, we can represent the state as a
-    mapping from identifiers to [nat].  For more complex programming
-    languages, the state might have more structure. *)
-
-Definition state := total_map nat.
+Inductive exp : Type :=
+  | Var : id -> exp
+  | ANum : nat -> exp
+  | APlus : exp -> exp -> exp
+  | AMinus : exp -> exp -> exp
+  | AMult : exp -> exp -> exp
+  | BTrue : exp
+  | BFalse : exp
+  | BEq : exp -> exp -> exp
+  | BLe : exp -> exp -> exp
+  | BNot : exp -> exp
+  | BAnd : exp -> exp -> exp.
+
+Definition state := partial_map nat.
 
 Definition empty_state : state :=
   t_empty 0.
@@ -1012,12 +179,12 @@ Definition empty_state : state :=
 (** We can add variables to the arithmetic expressions we had before by
     simply adding one more constructor: *)
 
-Inductive aexp : Type :=
-  | ANum : nat -> aexp
-  | AId : id -> aexp                (* <----- NEW *)
-  | APlus : aexp -> aexp -> aexp
-  | AMinus : aexp -> aexp -> aexp
-  | AMult : aexp -> aexp -> aexp.
+Inductive exp : Type :=
+  | ANum : nat -> exp
+  | AId : id -> exp                (* <----- NEW *)
+  | APlus : exp -> exp -> exp
+  | AMinus : exp -> exp -> exp
+  | AMult : exp -> exp -> exp.
 
 (** Defining a few variable names as notational shorthands will make
     examples easier to read: *)
@@ -1032,16 +199,16 @@ Definition Z : id := Id "Z".
     types.  Since we're not using polymorphism heavily in the chapters
     devoped to Imp, this overloading should not cause confusion.) *)
 
-(** The definition of [bexp]s is unchanged (except for using the new
-    [aexp]s): *)
+(** The definition of [exp]s is unchanged (except for using the new
+    [exp]s): *)
 
-Inductive bexp : Type :=
-  | BTrue : bexp
-  | BFalse : bexp
-  | BEq : aexp -> aexp -> bexp
-  | BLe : aexp -> aexp -> bexp
-  | BNot : bexp -> bexp
-  | BAnd : bexp -> bexp -> bexp.
+Inductive exp : Type :=
+  | BTrue : exp
+  | BFalse : exp
+  | BEq : exp -> exp -> exp
+  | BLe : exp -> exp -> exp
+  | BNot : exp -> exp
+  | BAnd : exp -> exp -> exp.
 
 (* ================================================================= *)
 (** ** Evaluation *)
@@ -1050,7 +217,7 @@ Inductive bexp : Type :=
     variables in the obvious way, taking a state as an extra
     argument: *)
 
-Fixpoint aeval (st : state) (a : aexp) : nat :=
+Fixpoint aeval (st : state) (a : exp) : nat :=
   match a with
   | ANum n => n
   | AId x => st x                                (* <----- NEW *)
@@ -1059,7 +226,7 @@ Fixpoint aeval (st : state) (a : aexp) : nat :=
   | AMult a1 a2 => (aeval st a1) * (aeval st a2)
   end.
 
-Fixpoint beval (st : state) (b : bexp) : bool :=
+Fixpoint beval (st : state) (b : exp) : bool :=
   match b with
   | BTrue       => true
   | BFalse      => false
@@ -1069,13 +236,13 @@ Fixpoint beval (st : state) (b : bexp) : bool :=
   | BAnd b1 b2  => andb (beval st b1) (beval st b2)
   end.
 
-Example aexp1 :
+Example exp1 :
   aeval (t_update empty_state X 5)
         (APlus (ANum 3) (AMult (AId X) (ANum 2)))
   = 13.
 Proof. reflexivity. Qed.
 
-Example bexp1 :
+Example exp1 :
   beval (t_update empty_state X 5)
         (BAnd BTrue (BNot (BLe (AId X) (ANum 4))))
   = true.
@@ -1117,15 +284,15 @@ Proof. reflexivity. Qed.
 
 Inductive com : Type :=
   | CSkip : com
-  | CAss : id -> aexp -> com
+  | CAss : id -> exp -> com
   | CSeq : com -> com -> com
-  | CIf : bexp -> com -> com -> com
-  | CWhile : bexp -> com -> com.
+  | CIf : exp -> com -> com -> com
+  | CWhile : exp -> com -> com.
 
 (** As usual, we can use a few [Notation] declarations to make things
     more readable.  To avoid conflicts with Coq's built-in notations,
     we keep this light -- in particular, we don't introduce any
-    notations for [aexps] and [bexps] to avoid confusion with the
+    notations for [exps] and [exps] to avoid confusion with the
     numeric and boolean operators we've already defined. *)
 
 Notation "'SKIP'" :=
@@ -1556,7 +723,7 @@ Proof.
       [12]          |
 
   The task of this exercise is to write a small compiler that
-  translates [aexp]s into stack machine instructions.
+  translates [exp]s into stack machine instructions.
 
   The instruction set for our stack language will consist of the
   following instructions:
@@ -1605,11 +772,11 @@ Example s_execute2 :
    = [15; 4].
 (* FILL IN HERE *) Admitted.
 
-(** Next, write a function that compiles an [aexp] into a stack
+(** Next, write a function that compiles an [exp] into a stack
     machine program. The effect of running the program should be the
     same as pushing the value of the expression on the stack. *)
 
-Fixpoint s_compile (e : aexp) : list sinstr
+Fixpoint s_compile (e : exp) : list sinstr
   (* REPLACE THIS LINE WITH ":= _your_definition_ ." *). Admitted.
 
 (** After you've defined [s_compile], prove the following to test
@@ -1634,7 +801,7 @@ Example s_compile1 :
     theorem will then be a simple corollary of this lemma. *)
 
 
-Theorem s_compile_correct : forall (st : state) (e : aexp),
+Theorem s_compile_correct : forall (st : state) (e : exp),
   s_execute st [] (s_compile e) = [ aeval st e ].
 Proof.
   (* FILL IN HERE *) Admitted.
@@ -1666,10 +833,10 @@ Module BreakImp.
 Inductive com : Type :=
   | CSkip : com
   | CBreak : com               (* <-- new *)
-  | CAss : id -> aexp -> com
+  | CAss : id -> exp -> com
   | CSeq : com -> com -> com
-  | CIf : bexp -> com -> com -> com
-  | CWhile : bexp -> com -> com.
+  | CIf : exp -> com -> com -> com
+  | CWhile : exp -> com -> com.
 
 Notation "'SKIP'" :=
   CSkip.
